simple load done :)

Registers.v
@@ -1,10 +1,25 @@
 From RecordUpdate Require Import RecordSet.
+Require Import Types.
+Import MixShort MixWord. (* TODO: why doesn't Import Types.MixWord work? *)
+Require Import Coq.ZArith.BinIntDef Coq.ZArith.BinInt.
+Local Open Scope Z_scope.
+
+Inductive reg : Type :=
+    (* general purpose *)
+    rA | rX
+    (* index registers *)
+    | rI1 | rI2 | rI3 | rI4 | rI5 | rI6
+    (* jump register *)
+    | rJ.
 
 Module Type Registers.
   Context (registers : Type).
+  Context (short : Type).
+  Context (word : Type).
   Context (zeroRegisters : registers).
-  Context (getReg : registers -> reg -> word + sign * byte * byte + byte * byte).
-  Context (setReg : registers -> reg -> word + sign * byte * byte + byte * byte -> registers).
+
+  Context (getReg : registers -> reg -> Z).
+  Context (setReg : registers -> reg -> Z -> registers).
 End Registers.
 
 Module MixRegisters : Registers.
@@ -28,12 +43,12 @@ Module MixRegisters : Registers.
                                     and two bytes: "...used primarily for
                                     for counting and for referencing
                                     variable memory addresses." *)
-                                 ; I1 : sign * byte * byte
-                                 ; I2 : sign * byte * byte
-                                 ; I3 : sign * byte * byte
-                                 ; I4 : sign * byte * byte
-                                 ; I5 : sign * byte * byte
-                                 ; I6 : sign * byte * byte
+                                 ; I1 : short
+                                 ; I2 : short
+                                 ; I3 : short
+                                 ; I4 : short
+                                 ; I5 : short
+                                 ; I6 : short
                                  (* Jump register comprised of two bytes
                                     and (TODO?) a sign, where the sign is
                                     always considered positive: "...always
@@ -41,61 +56,58 @@ Module MixRegisters : Registers.
                                     following the most recent 'jump'
                                     operation, and it is primarily used in
                                     connection with subroutines." *)
-                                 ; J : byte * byte
+                                 ; J : short
                                }.
   Definition registers : Type := registers'.
+
+  Definition short : Type := short.
+  Definition word : Type := word.
 
   (* For record updates *)
   Instance etaRegisters : Settable _ := settable! mkRegisters <A; X; I1; I2; I3; I4; I5; I6; J>.
 
+  Let zero_short := shortFromZ 0.
+  Let zero_word := shortFromZ 0.
+
   Definition zeroRegisters : registers := {| A := zero_word;
                                              X := zero_word;
-                                             I1 := (plus , zero_byte , zero_byte);
-                                             I2 := (plus , zero_byte , zero_byte);
-                                             I3 := (plus , zero_byte , zero_byte);
-                                             I4 := (plus , zero_byte , zero_byte);
-                                             I5 := (plus , zero_byte , zero_byte);
-                                             I6 := (plus , zero_byte , zero_byte);
-                                             J := (zero_byte , zero_byte); |}.
-  
+                                             I1 := zero_short;
+                                             I2 := zero_short;
+                                             I3 := zero_short;
+                                             I4 := zero_short;
+                                             I5 := zero_short;
+                                             I6 := zero_short;
+                                             J := zero_short; |}.
 
-  
-  Definition getReg (R : registers) (r : reg) : word + (sign * byte * byte) + (byte * byte) :=
-    match r with
-    | rA => inl (inl (A R))
-    | rX => inl (inl (X R))
-    | rI1 => inl (inr (I1 R))
-    | rI2 => inl (inr (I2 R))
-    | rI3 => inl (inr (I3 R))
-    | rI4 => inl (inr (I4 R))
-    | rI5 => inl (inr (I5 R))
-    | rI6 => inl (inr (I6 R))
-    | rJ => inr (J R)
-    end.
-  
+Print Registers.
+
+Print Word.
+Definition getReg (R : registers) (r : reg) : Z :=
+  match r with
+  | rA => signedFromWord (A R)
+  | rX => signedFromWord (X R)
+  | rI1 => signedFromShort (I1 R)
+  | rI2 => signedFromShort (I2 R)
+  | rI3 => signedFromShort (I3 R)
+  | rI4 => signedFromShort (I4 R)
+  | rI5 => signedFromShort (I5 R)
+  | rI6 => signedFromShort (I6 R)
+  | rJ => unsignedFromShort (J R) (* per Knuth, the jump register does have a sign, but we always ignore it *)
+  end.
+    
   Import RecordSetNotations.
-  Definition setReg (R : registers) (r : reg) (w : word + (sign * byte * byte) + (byte * byte) ) : registers :=
-    match w with
-    | inl (inl w) =>
-      match r with
-      | rA => R <|A := w|>
-      | rX => R <|X := w|>
-      | otherwise => R
-      end
-    | inl (inr s) =>
-      match r with
-        | rI1 => R <|I1 := s|>
-        | rI2 => R <|I2 := s|>
-        | rI3 => R <|I3 := s|>
-        | rI4 => R <|I4 := s|>
-        | rI5 => R <|I5 := s|>
-        | rI6 => R <|I6 := s|>
-        | _ => R
-      end
-    | inr s =>
-      match r with
-      | rJ => R <|J := s|>
-      | _ => R
-      end
+  Definition setReg (R : registers) (r : reg) (z : Z) : registers :=
+    let w := wordFromZ z in
+    let s := shortFromZ z in 
+    match r with
+    | rA => R <|A := w|>
+    | rX => R <|X := w|>
+    | rI1 => R <|I1 := s|>
+    | rI2 => R <|I2 := s|>
+    | rI3 => R <|I3 := s|>
+    | rI4 => R <|I4 := s|>
+    | rI5 => R <|I5 := s|>
+    | rI6 => R <|I6 := s|>
+    | rJ => R <|J := s|>
     end.
 End MixRegisters.
