machine.v
@@ -2,115 +2,8 @@ Require Import Omega.
 Require Import Finite.
 From RecordUpdate Require Import RecordSet.
 Require Import Types.
-Import MixWord.
-
-Inductive reg : Type :=
-    (* general purpose *)
-    rA | rX
-    (* index registers *)
-    | rI1 | rI2 | rI3 | rI4 | rI5 | rI6
-    (* jump register *)
-    | rJ.
-
-Module Type Registers.
-  Context (registers : Type).
-  Context (zeroRegisters : registers).
-  Context (getReg : registers -> reg -> word).
-  Context (setReg : registers -> reg -> word -> registers).
-End Registers.
-
-Module MixRegisters : Registers.
-  (* Dumb coq bug: the kernel won't let you instantiate a parameter
-     with an record type (nor with an inductive definition)
-     directly. *)
-  Record registers' : Type := mkRegisters 
-                               {
-                                 (* Accumulator: "...has many uses,
-                                    especially for arithmetic and operating
-                                    on data." *)
-                                 A : word
-                                 (* Extension register: "...an extension
-                                    on the 'right-hand side' of rA, and it
-                                    is is used in conjuction with rA to hold
-                                    ten bytes of a product or dividend, or
-                                    it can be used to hold information
-                                    shifted to the right out of A." *)
-                                 ; X : word
-                                 (* Index registers comprised of a sign
-                                    and two bytes: "...used primarily for
-                                    for counting and for referencing
-                                    variable memory addresses." *)
-                                 ; I1 : sign * byte * byte
-                                 ; I2 : sign * byte * byte
-                                 ; I3 : sign * byte * byte
-                                 ; I4 : sign * byte * byte
-                                 ; I5 : sign * byte * byte
-                                 ; I6 : sign * byte * byte
-                                 (* Jump register comprised of two bytes
-                                    and (TODO?) a sign, where the sign is
-                                    always considered positive: "...always
-                                    holds the address of the instruction
-                                    following the most recent 'jump'
-                                    operation, and it is primarily used in
-                                    connection with subroutines." *)
-                                 ; J : byte * byte
-                               }.
-  Definition registers : Type := registers'.
-
-  (* For record updates *)
-  Instance etaRegisters : Settable _ := settable! mkRegisters <A; X; I1; I2; I3; I4; I5; I6; J>.
-
-  Definition zeroRegisters : registers := {| A := zero_word;
-                                             X := zero_word;
-                                             I1 := (plus , zero_byte , zero_byte);
-                                             I2 := (plus , zero_byte , zero_byte);
-                                             I3 := (plus , zero_byte , zero_byte);
-                                             I4 := (plus , zero_byte , zero_byte);
-                                             I5 := (plus , zero_byte , zero_byte);
-                                             I6 := (plus , zero_byte , zero_byte);
-                                             J := (zero_byte , zero_byte); |}.
-  
-
-  
-  Definition getReg (R : registers) (r : reg) : word + (sign * byte * byte) + (byte * byte) :=
-    match r with
-    | rA => inl (inl (A R))
-    | rX => inl (inl (X R))
-    | rI1 => inl (inr (I1 R))
-    | rI2 => inl (inr (I2 R))
-    | rI3 => inl (inr (I3 R))
-    | rI4 => inl (inr (I4 R))
-    | rI5 => inl (inr (I5 R))
-    | rI6 => inl (inr (I6 R))
-    | rJ => inr (J R)
-    end.
-  
-  Import RecordSetNotations.
-  Definition setReg (R : registers) (r : reg) (w : word + (sign * byte * byte) + (byte * byte) ) : registers :=
-    match w with
-    | inl (inl w) =>
-      match r with
-      | rA => R <|A := w|>
-      | rX => R <|X := w|>
-      | otherwise => R
-      end
-    | inl (inr s) =>
-      match r with
-        | rI1 => R <|I1 := s|>
-        | rI2 => R <|I2 := s|>
-        | rI3 => R <|I3 := s|>
-        | rI4 => R <|I4 := s|>
-        | rI5 => R <|I5 := s|>
-        | rI6 => R <|I6 := s|>
-        | _ => R
-      end
-    | inr s =>
-      match r with
-      | rJ => R <|J := s|>
-      | _ => R
-      end
-    end.
-End MixRegisters.
+Require Import Registers.
+Import MixShort MixWord.
 
 Record flags : Type := mkFlags 
                          {
@@ -131,10 +24,9 @@ Definition zeroFlags : flags := {| comparison := Eq;
 Context (size : nat).
 Context (Hsizenontrivial : size > 0).
 
-Definition address : Type := fin size.
+Definition address : Type := {n : nat | n < size}.
 
 Module Type Memory.
-  Context {size : nat}.
   Context (memory : Type).
   Context (zeroMemory : memory).
   Context (HMemNontrivial : size > 0).
@@ -146,8 +38,8 @@ End Memory.
 Module MixMemory : Memory.
   (* Each MIX machine has a 4000-word memory. We represent this in
      Coq as a finite map from a type with 4000 inhabitants to words. *)
-  Definition size := size.
   Definition memory := fin size -> word.
+  Let zero_word := wordFromZ 0.
   Definition zeroMemory : memory := fun n => zero_word.
   Definition HMemNontrivial : size > 0.
     exact Hsizenontrivial.
@@ -178,9 +70,9 @@ Defined.
 
 Open Scope list_scope.
 
-Definition fieldspecToByte F := natToByte (fieldspecToNat F).
-
 Import MixRegisters.
+
+Definition sign := bool.
 
 Inductive instruction : Type :=
 (** * Loads and stores *)
@@ -198,13 +90,13 @@ register. *)
 | Mul : address -> option fieldspec -> instruction
 | Div : address -> option fieldspec -> instruction
                                        
-(** * Address transfer operations *)
+(** * address transfer operations *)
 (* Enter a word, optionally negating it and optionally adjusted by the value in a given index register, into a register *)
-| Ent : sign -> reg -> word -> option reg -> instruction
+| Ent : sign -> reg -> Z -> option reg -> instruction
 (* increase the value contained in a given register by a given word *)
-| Inc : reg -> word -> instruction
+| Inc : reg -> Z -> instruction
 (* decrease the value contained in a given register by a given word *)
-| Dec : reg -> word -> instruction
+| Dec : reg -> Z -> instruction
 
 (** * Comparison operators *)
 | Cmp : reg -> address -> fieldspec -> instruction
@@ -238,14 +130,14 @@ register. *)
 (** * Miscellaneous operators *)
 (** shifts *)
 (* Shift a given register left or right by a given number of bytes *)
-| Sl : reg -> word -> instruction
-| Sr : reg -> word -> instruction
+| Sl : reg -> nat -> instruction
+| Sr : reg -> nat -> instruction
 (* special AX-shifts *)
-| Slax : word -> instruction
-| Srax : word -> instruction
+| Slax : nat -> instruction
+| Srax : nat -> instruction
 (* circular AX-shifts *)
-| Slc : word -> instruction
-| Src : word -> instruction
+| Slc : nat -> instruction
+| Src : nat -> instruction
 
 (* Move the number of words specified by the fieldspec from location M
    to the location specified by the contents of I1 *)
@@ -261,7 +153,7 @@ register. *)
           
 (** * TODO: Conversion operators *)
 (* Left for later due to laziness *).
-
+Import Registers.
 Import MixMemory.
 
 Record machine : Type := mkMachine {
@@ -288,24 +180,43 @@ Inductive instWf : instruction -> Prop :=
     instWf (Load sign rDest from maybeIndex maybeFieldspec)
 | HaltWf : instWf Hlt.
 
+(* For record updates *)
+Instance etaMachine : Settable _ := settable! mkMachine <r; f; m>.
+Import RecordSetNotations.
+
+
+
+Search "set".
+
+Check (fun (r' : registers -> registers) (m : machine) => set r r' m).
+
+Search "setReg".
+Search "word".
 Definition instDenote (M : machine) (I : {I : instruction | instWf I}) : machine :=
   let (I, _) := I in 
-    in match I with
-       | (Load sign rDest from maybeIndex maybeFieldspec, _) =>
-         match (maybeIndex, maybeFieldspec) with
-         | (Some(I), Some(F)) =>
-           (* offset from by the value contained in I *)
-           let offset := indexToNat (getReg I) in
-         | (Some(I), None) => 
-         | (None, Some(F)) =>
-         | (None, None) => 
-           let 
-             {| r := 
-                  f := M.f;
-                m := M.m;
-             |}
-           | otherwise => M
-             end.
+  match I with
+  | Load sign rDest from maybeIndex maybeFieldspec =>
+    let fromVal := signedFromWord (get_nth_cell (m M) from)
+    in let newReg := setReg (r M) rDest fromVal
+       in
+       M <| r := newReg |>
+  | _ => M
+  end.
+
+    match (maybeIndex, maybeFieldspec) with
+    | (Some(I), Some(F)) =>
+      (* offset from by the value contained in I *)
+      let offset := indexToNat (getReg I) in
+    | (Some(I), None) => 
+    | (None, Some(F)) =>
+    | (None, None) => 
+      let 
+        {| r := 
+             f := M.f;
+           m := M.m;
+        |}
+      | otherwise => M
+        end.
 
 Definition Halto : {I : instruction | instWf I}.
   econstructor.
